Environment composition. Refactoring.

coq/Env.v
@@ -1,197 +1,264 @@
 Require Import Coq.Arith.EqNat.
 Require Import Coq.Lists.List.
+Require Import Coq.Classes.RelationClasses.
 Require Import Cases.
-Require Import Patt.
 
+Module Type VALUE.
+  Parameter val : Type.
+  Parameter var : Type.
+  Parameter beq_var : var -> var -> bool.
 
-Inductive env :=
-| mtEnv : env
-| bind : vid -> term -> env -> env.
+  Parameter beq_var_refl : forall (v : var),
+    beq_var v v = true.
+  Parameter beq_var_sym : forall (x y : var),
+    beq_var x y = beq_var y x.
+  Parameter beq_var_trans : forall (x y z : var),
+    beq_var x y = true -> beq_var y z = true -> beq_var x z = true.
+End VALUE.
 
-Fixpoint try_lookup (v : vid) (e : env) : option term :=
-  match e with
-    | mtEnv => None
-    | bind v' t e =>
-      if beq_vid v v'
-        then Some t
-        else try_lookup v e
-  end.
+Module ENV (Import Value : VALUE).
 
-Definition lookup (v : vid) (e : env) : patt :=
-  match try_lookup v e with
-    | None => pvar v
-    | Some t => term_to_patt t
-  end.
+  Require Import Coq.Setoids.Setoid Coq.Classes.SetoidClass.
 
-Definition bmem (v : vid) (e : env) : bool :=
-  match try_lookup v e with
-    | None => false
-    | Some _ => true
-  end.
+  Definition beq_var_eq v1 v2 := beq_var v1 v2 = true.
+  Lemma beq_var_eq_refl : forall v, beq_var_eq v v. 
+  Proof. apply beq_var_refl. Qed.
+  Lemma beq_var_eq_sym : forall v1 v2, beq_var_eq v1 v2 -> beq_var_eq v2 v1.
+  Proof. intros. unfold beq_var_eq. rewrite beq_var_sym. auto. Qed.
+  Lemma beq_var_eq_trans : forall v1 v2 v3, beq_var_eq v1 v2 -> beq_var_eq v2 v3 -> beq_var_eq v1 v3.
+  Proof. unfold beq_var_eq; intros. apply beq_var_trans with v2; auto. Qed.
+  Add Relation var beq_var_eq
+  reflexivity proved by beq_var_eq_refl
+  symmetry proved by beq_var_eq_sym
+    transitivity proved by beq_var_eq_trans
+    as Beq_var.
 
-Definition mem (v : vid) (e : env) : Prop :=
-  bmem v e = true.
+  Instance Beq_var_Setoid : Setoid var :=
+    {equiv := beq_var_eq; setoid_equiv := Beq_var}.
 
-Fixpoint insert_binding (v : vid) (t : term) (e : env) : option env :=
-  match e with
-    | mtEnv => Some (bind v t mtEnv)
-    | bind v' t' e' =>
-      if beq_vid v v'
-        then None
-        else match insert_binding v t e' with
-               | None => None
-               | Some e' => Some (bind v' t' e')
-             end
-  end.
+  Require Import Coq.Logic.Decidable.
+  Lemma beq_var_eq_dec : forall v1 v2, decidable (v1 == v2).
+  Proof. unfold decidable. intros. destruct (beq_var v1 v2) eqn:v1v2. 
+    left; auto. rewrite <- Bool.not_true_iff_false in v1v2. right; auto.
+  Qed.
 
-(* Compose two environments. Fail if they overlap. *)
-Fixpoint compose_env (e1 e2 : env) {struct e1} : option env :=
-  match e1 with
-    | mtEnv => Some e2
-    | bind v t e1 =>
-      if bmem v e2
-        then None
-        else match compose_env e1 e2 with
-               | None => None
-               | Some e => Some (bind v t e)
-             end
-  end.
+  Inductive env :=
+  | mtEnv : env
+  | bind : var -> val -> env -> env.
 
-Notation "x & y" := (compose_env x y) (at level 60).
+  Fixpoint lookup (v : var) (e : env) : option val :=
+    match e with
+      | mtEnv => None
+      | bind v' t e =>
+        if beq_var v v'
+          then Some t
+          else lookup v e
+    end.
 
-Fixpoint subs (e : env) (p : patt) : patt :=
-  match p with
-    | pvar v => lookup v e
-    | pnode n ps => pnode n (map (subs e) ps)
-  end.
+  Definition env_eqv (e1 e2 : env) :=
+    forall (v : var), lookup v e1 = lookup v e2.
 
-Notation "e * p" := (subs e p).
+  Lemma env_eqv_refl : forall e, env_eqv e e. 
+  Proof. unfold env_eqv. reflexivity. Qed.
+  Lemma env_eqv_sym : forall e f, env_eqv e f -> env_eqv f e.
+  Proof. unfold env_eqv. intros. symmetry; auto. Qed.
+  Lemma env_eqv_trans : forall e f g, env_eqv e f -> env_eqv f g -> env_eqv e g.
+  Proof. unfold env_eqv. intros. rewrite H; auto. Qed.
 
-Definition env_eqv (e1 e2 : env) :=
-  forall (v : vid), lookup v e1 = lookup v e2.
+  Add Relation env env_eqv
+  reflexivity proved by env_eqv_refl
+  symmetry proved by env_eqv_sym
+    transitivity proved by env_eqv_trans
+    as Env_eqv.
 
-Notation "e1 ~= e2" := (env_eqv e1 e2) (at level 40).
+  Instance env_eqv_Setoid : Setoid env :=
+    {equiv := env_eqv; setoid_equiv := Env_eqv}.
 
+  Add Parametric Morphism : lookup with signature (equiv ==> equiv ==> eq) as Lookup_beq_var.
+  Proof.
+    intros. generalize dependent x0; induction y0; intros x0 H0; rewrite H0; auto.
+    simpl. destruct (beq_var x v) eqn:xv; destruct (beq_var y v) eqn:yv;
+    try change (x == v) in xv; try change (y == v) in yv; try rewrite <- Bool.not_true_iff_false in *;
+    try change (y =/= v) in yv; try change (x =/= v) in xv; auto. 
+    rewrite <- xv in yv. 
+    symmetry in H; contradiction. rewrite <- yv in xv; contradiction.
+    apply IHy0. reflexivity.
+  Qed.
 
+  Definition bmem (v : var) (e : env) : bool :=
+    match lookup v e with
+      | None => false
+      | Some _ => true
+    end.
 
+  Add Parametric Morphism : bmem with signature (equiv ==> equiv ==> eq) as bmem_beq_var.
+  Proof.
+    unfold bmem. intros. rewrite H. rewrite H0. reflexivity.
+  Qed.
+
+  Definition mem (v : var) (e : env) : Prop :=
+    bmem v e = true.
+
+  Add Parametric Morphism : mem with signature (equiv ==> equiv ==> eq) as mem_beq_var.
+  Proof.
+    unfold mem; intros; rewrite H; rewrite H0; reflexivity.
+  Qed.
+
+  (* Disjoint union *)
+  Fixpoint union (e1 e2 : env) {struct e1} : option env :=
+    match e1 with
+      | mtEnv => Some e2
+      | bind v t e1 =>
+        if bmem v e2
+          then None
+          else match union e1 e2 with
+                 | None => None
+                 | Some e => Some (bind v t e)
+               end
+    end.
+  Notation "x & y" := (union x y) (at level 60).
+
+  (* Juxtposition *)
+  Fixpoint concat (e1 e2 : env) : env :=
+    match e1 with
+      | mtEnv => e2
+      | bind v t e => bind v t (concat e e2)
+    end.
+  Notation "e1 ++ e2" := (concat e1 e2).
 
 (*******************)
 (*** Easy Lemmas ***)
 (*******************)
 
+  Lemma mem_mtEnv : forall (v : var), ~ (mem v mtEnv).
+  Proof. intros. unfold mem. simpl. exact (Bool.diff_false_true). Qed.
 
+  Lemma mem__mem_bind : forall (v v' : var) (t : val) (e : env),
+    mem v e -> mem v (bind v' t e).
+  Proof.
+    intros.
+    unfold mem, bmem, lookup in *.
+    destruct (beq_var v v'); auto.
+  Qed.
 
-Lemma env_eqv_subs : forall (e1 e2 : env) (p : patt),
-  e1 ~= e2 -> e1 * p = e2 * p.
-Proof.
-  intros. induction p.
-  Case "var v". simpl. unfold env_eqv in H. apply H.
-  Case "node n nil". reflexivity.
-  Case "node n (p :: ps)". simpl. rewrite IHp.
-    inversion IHp0. rewrite H1. reflexivity.
-Qed.
+  Lemma mem_bind : forall v t e, mem v (bind v t e).
+  Proof.
+    intros. unfold mem, bmem, lookup.
+    rewrite beq_var_refl. reflexivity.
+  Qed.
 
-Lemma mtEnv_subs_l : forall (p : patt), mtEnv * p = p.
-Proof.
-  intros. induction p; try reflexivity.
-  Case "node n (p :: ps)". inversion IHp0.
-    simpl. rewrite IHp. rewrite H0. rewrite H0. reflexivity.
-Qed.
+  Lemma mem_bind_same : forall (v v' : var) (t : val) (e : env),
+    v == v' -> mem v (bind v' t e).
+  Proof.
+    intros. unfold mem. rewrite H. unfold bmem. simpl. rewrite beq_var_refl; auto.
+  Qed.
 
-Lemma mem_mtEnv : forall (v : vid), ~ (mem v mtEnv).
-Proof. intros. unfold mem. simpl. exact (Bool.diff_false_true). Qed.
+  Lemma mem_bind_diff : forall (v v' : var) (t : val) (e : env),
+    v =/= v' -> mem v (bind v' t e) -> mem v e.
+  Proof.
+    intros. unfold mem in *. unfold bmem in *. simpl in H0.
+    destruct (beq_var v v') eqn:vv'. contradiction. auto.
+  Qed.
 
-Lemma beq_vid_sym : forall (v v' : vid),
-  beq_vid v v' = beq_vid v' v.
-Proof. intros. unfold beq_vid. apply NPeano.Nat.eqb_sym. Qed.
+  Lemma bmem_true : forall (v : var) (e : env),
+    bmem v e = true -> mem v e.
+  Proof. intros. unfold mem. exact H. Qed.
 
-Lemma mem_bind : forall (v v' : vid) (t : term) (e : env),
-  mem v e -> mem v (bind v' t e).
-Proof.
-  intros. unfold mem. unfold bmem. unfold try_lookup.
-  unfold mem in H. unfold bmem in H. unfold try_lookup in H.
-  destruct (beq_vid v v').
-    reflexivity.
-    exact H.
-Qed.
-
-Lemma mem_bind_same : forall (v v' : vid) (t : term) (e : env),
-  beq_vid v v' = true -> mem v' (bind v t e).
-Proof.
-  intros. unfold beq_vid in H. apply beq_nat_true in H. rewrite H.
-  unfold mem. unfold bmem. simpl. rewrite beq_vid_refl. reflexivity.
-Qed.
-
-Lemma mem_bind_diff : forall (v v' : vid) (t : term) (e : env),
-  beq_vid v v' = false -> mem v (bind v' t e) -> mem v e.
-Proof.
-  intros. unfold mem in *. unfold bmem in *. unfold try_lookup in *.
-  unfold beq_vid in *. rewrite H in H0. exact H0.
-Qed.
-
-Lemma mem_bind_same' : forall (v : vid) (t : term) (e : env),
-  mem v (bind v t e).
-Proof.
-  intros. unfold mem. unfold bmem. simpl.
-  rewrite beq_vid_refl. reflexivity.
-Qed.
-
-Lemma bmem_true : forall (v : vid) (e : env),
-  bmem v e = true -> mem v e.
-Proof. intros. unfold mem. exact H. Qed.
-
-Lemma bmem_false : forall (v : vid) (e : env),
-  bmem v e = false -> ~ (mem v e).
-Proof.
-  intros. unfold mem. destruct (bmem v e).
+  Lemma bmem_false : forall (v : var) (e : env),
+    bmem v e = false -> ~ (mem v e).
+  Proof.
+    intros. unfold mem. destruct (bmem v e).
     inversion H.
     exact Bool.diff_false_true.
-Qed.
+  Qed.
 
-Lemma lookup_bind : forall (v : vid) (t : term) (e : env),
-  lookup v (bind v t e) = term_to_patt t.
-Proof.
-  intros. unfold lookup. unfold try_lookup.
-  rewrite beq_vid_refl. reflexivity.
-Qed.
+  Lemma lookup_bind_same : forall (v v' : var) (t : val) (e : env),
+    v == v' -> lookup v (bind v' t e) = Some t.
+  Proof.
+    intros. unfold lookup.
+    rewrite H. reflexivity.
+  Qed.
 
-Lemma lookup_bind_same : forall (v v' : vid) (t : term) (e : env),
-  beq_vid v v' = true -> lookup v (bind v' t e) = term_to_patt t.
-Proof.
-  intros. unfold lookup. unfold try_lookup.
-  rewrite H. reflexivity.
-Qed.
+  Lemma lookup_bind_diff : forall (v v' : var) (t : val) (e : env),
+    v =/= v' -> lookup v (bind v' t e) = lookup v e.
+  Proof.
+    intros. unfold lookup. destruct (beq_var v v') eqn:vv'. 
+    change (v == v') in vv'; contradiction. reflexivity.
+  Qed.
 
-Lemma lookup_bind_diff : forall (v v' : vid) (t : term) (e : env),
-  beq_vid v v' = false -> lookup v (bind v' t e) = lookup v e.
-Proof.
-  intros. unfold lookup. unfold try_lookup.
-  rewrite H. reflexivity.
-Qed.
 
-Lemma mem__subs_closed : forall (v : vid) (e : env),
-  mem v e -> closed (e * (pvar v)).
-Proof.
-  intros. simpl.
-  unfold mem in H. unfold bmem in H.
-  unfold lookup. destruct (try_lookup v e).
-  Case "v in e".
-    apply term_to_patt_closed. inversion H.
-Qed.
+(*********************)
+(*** Concat Lemmas ***)
+(*********************)
 
-Lemma closed_subs : forall (p : patt) (e : env),
-  closed p -> e * p = p.
-Proof.
-  intros. induction p.
-  Case "var". inversion H.
-  Case "node n nil". reflexivity.
-  Case "node n (p :: ps)". simpl in *.
-    inversion H; clear H.
-    apply IHp in H0; clear IHp. rewrite H0.
-    apply IHp0 in H1; clear IHp0. inversion H1.
-      rewrite H2. rewrite H2. reflexivity.
-Qed.
 
+  Lemma lookup_concat_member : forall (v : var) (e1 e2 : env) (x : val),
+    lookup v e1 = Some x -> lookup v (e1 ++ e2) = Some x.
+  Proof.
+    intros. generalize dependent e2. induction e1 as [|v1 t1 e1].
+    Case "mtEnv".
+      simpl in H. inversion H.
+    Case "bind v1 t1 e2".
+      intros. simpl in *. destruct (beq_var v v1).
+      SCase "v == v1". exact H.
+      SCase "v /= v1". apply IHe1. exact H.
+  Qed.
+
+  Lemma lookup_concat_not_member : forall (v : var) (e1 e2 : env),
+    ~ (mem v e1) -> lookup v (e1 ++ e2) = lookup v e2.
+  Proof.
+    intros. generalize dependent e2. induction e1 as [|v1 t1 e1].
+    Case "mtEnv".
+      intros. simpl. reflexivity.
+    Case "bind v1 t1 e1".
+      intros. unfold mem in *. unfold bmem in *. simpl in *.
+      destruct (beq_var v v1).
+      SCase "v == v1". tauto.
+      SCase "v /= v1".
+        apply IHe1. exact H.
+  Qed.
+
+  Lemma lookup_mem : forall e v, (exists t, lookup v e = Some t) <-> mem v e.
+  Proof. unfold mem. unfold bmem. intros; destruct (lookup v e) eqn:ve; auto.
+    split; eauto. 
+    split; intro; eauto. inversion H. inversion H0. inversion H.
+  Qed.
+
+  Lemma lookup_not_member : forall (v : var) (e : env),
+    ~ (mem v e) <-> lookup v e = None.
+  Proof.
+    intros; split. intros.
+    destruct (lookup v e) eqn:ve; auto. unfold mem in H. unfold bmem in H.
+    rewrite ve in H. tauto.
+    intro; intro. rewrite <- lookup_mem in H0. inversion H0.
+    rewrite H1 in H. inversion H.
+  Qed.
+
+  Lemma concat_comm_equiv : forall e1 e2 e12, e1 & e2 = Some e12 -> (e1 ++ e2) == (e2 ++ e1).
+  Proof.
+    cut (forall e1 e2, (exists e12, e1 & e2 = Some e12) -> (e1 ++ e2) == (e2 ++ e1)).
+    intros. assert (exists e, e1 & e2 = Some e) by (exists e12; auto). apply H; auto.
+    intros.
+    induction e1. 
+    Case "e1 = mtEnv". simpl; intro. symmetry.
+    destruct (lookup v e2) eqn:ve2. 
+    apply lookup_concat_member with _ _ mtEnv _ in ve2; auto.
+    apply lookup_concat_not_member. apply lookup_not_member. auto.
+    Case "e1 <> mtEnv".
+    inversion_clear H as (e12 & H1). simpl in H1.
+    destruct (bmem v e2) eqn:ve2; try discriminate.
+    destruct (e1 & e2) eqn:e12'; try discriminate. clear H1.
+    assert (exists e12, Some e = Some e12) by (exists e; auto). 
+    apply IHe1 in H. intro. simpl. rewrite H. 
+    destruct (beq_var_eq_dec v1 v). repeat rewrite H0 in *. 
+    rewrite lookup_concat_not_member. rewrite lookup_bind_same; reflexivity.
+    apply bmem_false; auto.
+    assert (beq_var v1 v = false) by (apply Bool.not_true_iff_false; auto).
+    rewrite H1.
+    destruct (lookup v1 e2) eqn:v1e2. 
+    repeat erewrite lookup_concat_member; eauto.
+    repeat (rewrite lookup_concat_not_member; simpl); try apply lookup_not_member; try rewrite H1; auto.
+  Qed.
 
 
 (**************************)
@@ -200,222 +267,198 @@ Qed.
 
 
 
-Lemma compose_mtEnv_l : forall (e : env), mtEnv & e = Some e.
-Proof. reflexivity. Qed.
+  Lemma compose_mtEnv_l : forall (e : env), mtEnv & e = Some e.
+  Proof. reflexivity. Qed.
 
-Lemma compose_mtEnv_r : forall (e : env), e & mtEnv = Some e.
-Proof.
-  intros. induction e.
-  Case "mtEnv". reflexivity.
-  Case "bind v t e". simpl. rewrite IHe. reflexivity.
-Qed.
+  Lemma compose_mtEnv_r : forall (e : env), e & mtEnv = Some e.
+  Proof.
+    intros. induction e.
+    Case "mtEnv". reflexivity.
+    Case "bind v t e". simpl. rewrite IHe. reflexivity.
+  Qed.
 
-Lemma bind_compose :
-  forall (v : vid) (t : term) (e1 e2 e12: env),
-  (bind v t e1) & e2 = Some e12 ->
-  exists e12', e1 & e2 = Some e12' /\ e12 = bind v t e12'.
-Proof.
-  intros. unfold compose_env in H. fold compose_env in H.
-  destruct (bmem v e2).
-  Case "true". inversion H.
-  Case "false". destruct (e1 & e2).
-    SCase "Some e". exists e. split.
-      reflexivity.
-      inversion H. reflexivity.
-    SCase "None". inversion H.
-Qed.
+  Lemma bind_compose :
+    forall (v : var) (t : val) (e1 e2 e12: env),
+      (bind v t e1) & e2 = Some e12 ->
+      exists e12', e1 & e2 = Some e12' /\ e12 = bind v t e12'.
+  Proof.
+    intros. simpl in H.
+    destruct (bmem v e2).
+    Case "true". inversion H.
+    Case "false". destruct (e1 & e2); inversion H.
+    SCase "Some e". exists e; split; auto.
+  Qed.
 
-Lemma compose_overlap : forall (e1 e2 : env) (v : vid),
-  mem v e1 -> mem v e2 -> e1 & e2 = None.
-Proof.
-  intros.
-  induction e1 as [ | v1 t e1].
-  Case "mtEnv". simpl in *. inversion H.
-  Case "bind v1 t1 e1". intros.
-    unfold compose_env.
-    destruct (bmem v1 e2) eqn:M; try reflexivity.
-    fold compose_env.
-    destruct (e1 & e2); try reflexivity.
-    destruct (beq_vid v v1) eqn:V.
+
+  Lemma beq_var_mem : forall (v1 v2 : var) (e : env),
+    v1 == v2 -> (mem v1 e <-> mem v2 e).
+  Proof.
+    intros. rewrite H. split; auto.
+  Qed.
+
+  Lemma compose_overlap : forall (e1 e2 : env) (v : var),
+    mem v e1 -> mem v e2 -> e1 & e2 = None.
+  Proof.
+    intros.
+    induction e1 as [ | v1 t e1].
+    Case "mtEnv". simpl in *. inversion H.
+    Case "bind v1 t1 e1". simpl.
+      destruct (bmem v1 e2) eqn:M; try reflexivity. unfold mem in H0. 
+      destruct (e1 & e2); try reflexivity.
+      destruct (beq_var_eq_dec v v1).
     SCase "v == v1".
-      apply beq_vid_true in V; subst.
-      apply bmem_false in M. elim M; apply H0.
+      repeat rewrite H1 in *. rewrite H0 in M; inversion M. 
     SCase "v != v1".
-      apply (mem_bind_diff v v1 t e1) in V.
-        apply IHe1 in V; inversion V.
-        exact H.
-Qed.
+      apply (mem_bind_diff v v1 t e1 H1) in H. apply IHe1 in H. inversion H.
+  Qed.
+  Hint Resolve compose_overlap.
 
-Lemma compose_not_member : forall (e1 e2 e12 : env) (v : vid),
-  ~ (mem v e1) ->
-  e1 & e2 = Some e12 ->
-  lookup v e12 = lookup v e2.
-Proof.
-  intros.
-  generalize dependent e12.
-  induction e1 as [ | v1 t e1]; intros.
-  Case "mtEnv".
-    simpl in H0. inversion H0. reflexivity.
-  Case "bind v1 t e1". intros.
-    apply bind_compose in H0.
-    elim H0; intros; rename x into e; clear H0.
-    inversion H1; clear H1. subst.
-    destruct (beq_vid v v1) eqn:V.
-    SCase "v == v1".
-      elim H. apply mem_bind_same. rewrite beq_vid_sym. exact V.
-    SCase "v /= v1".
-      rewrite lookup_bind_diff.
-        apply IHe1; clear IHe1.
-          intro. elim H. apply mem_bind. exact H1.
-          exact H0.
-        exact V.
-Qed.
+  Lemma compose_overlap_2 : forall e1 e2,
+    e1 & e2 = None -> (exists v, mem v e1 /\ mem v e2).
+  Proof.
+    induction e1; intros. inversion H.
+    simpl in H. destruct (bmem v e2) eqn:ve2.
+    exists v. split; unfold mem; unfold bmem; simpl; try rewrite beq_var_refl; auto.
+    destruct (e1 & e2) eqn:e12. inversion H. apply IHe1 in e12. inversion e12 as (x & H1 & H2). 
+    exists x; split; auto. apply mem__mem_bind; auto.
+  Qed.
 
-Lemma lookup_mtEnv : forall (v : vid), lookup v mtEnv = pvar v.
-Proof. intros. compute. reflexivity. Qed.
+  Lemma compose_overlap_3 : forall e1 e2 e12,
+    e1 & e2 = Some e12 -> ~ exists v, mem v e1 /\ mem v e2.
+  Proof.
+    intros. intro. inversion H0 as (v & H1 & H2). assert (H3 := compose_overlap _ _ _ H1 H2).
+    inversion H. rewrite H3 in H5; inversion H5.
+  Qed.
 
-Lemma lookup_not_member : forall (v : vid) (e : env),
-  ~ (mem v e) -> lookup v e = pvar v.
-Proof.
-  intros.
-  assert (e & mtEnv = Some e).
-    rewrite compose_mtEnv_r. reflexivity.
-  assert (lookup v e = lookup v mtEnv).
-    apply compose_not_member with (e1 := e). exact H. exact H0.
-  rewrite H1. rewrite lookup_mtEnv. reflexivity.
-Qed.
+  Lemma compose_not_member : forall (e1 e2 e12 : env) (v : var),
+    e1 & e2 = Some e12 ->
+    ~ (mem v e1) ->
+    lookup v e12 = lookup v e2.
+  Proof.
+    intros.
+    generalize dependent e12.
+    induction e1 as [ | v1 t e1]; intros.
+    Case "mtEnv".
+      simpl in H. inversion H. reflexivity.
+    Case "bind v1 t e1".
+      assert (~ mem v e1). intro; apply H0. apply mem__mem_bind; auto.
+      simpl in H. destruct (bmem v1 e2) eqn:v1e2; try discriminate.
+      destruct (e1 & e2); try discriminate.
+      inversion_clear H. simpl. destruct (beq_var v v1) eqn:vv1.
+      unfold mem in H0. unfold bmem in H0. simpl in H0. rewrite vv1 in H0. tauto. 
+      apply IHe1; auto.
+  Qed.
+  Hint Resolve compose_not_member.
 
-Lemma compose_lookup_l : forall (e1 e2 e12 : env) (v : vid),
-  mem v e1 ->
-  e1 & e2 = Some e12 ->
-  lookup v e12 = lookup v e1.
-Proof.
-  intros.
-  generalize dependent e2. generalize dependent e12.
-  induction e1 as [ | v1 t e1].
-  Case "mtEnv".
-    apply mem_mtEnv in H. inversion H.
-  Case "bind v1 t1 e1". intros.
-    apply bind_compose in H0.
-    elim H0; intros; rename x into e; clear H0.
-    inversion H1; clear H1. subst.
-    destruct (beq_vid v v1) eqn:V.
-    SCase "v == v1".
-      rewrite (lookup_bind_same v v1 t e1 V).
-      rewrite (lookup_bind_same v v1 t e V).
-      reflexivity.
-    SCase "v /= v1".
-      rewrite (lookup_bind_diff v v1 t e1 V).
-      rewrite (lookup_bind_diff v v1 t e V).
-      apply IHe1 with (e2 := e2).
-      apply mem_bind_diff with (v' := v1) (t := t).
-        exact V. exact H. exact H0.
-Qed.
+  Lemma lookup_mtEnv : forall (v : var), lookup v mtEnv = None.
+  Proof. intros. compute. reflexivity. Qed.
 
-Lemma compose_lookup_r : forall (e1 e2 e12 : env) (v : vid),
-  mem v e2 ->
-  compose_env e1 e2 = Some e12 ->
-  lookup v e12 = lookup v e2.
-Proof.
-  intros.
-  generalize dependent e2. generalize dependent e12.
-  induction e1 as [ | v1 t e1].
-  Case "mtEnv". intros.
-    inversion H0. reflexivity.
-  Case "bind v1 t e1". intros.
-    destruct (beq_vid v v1) eqn:V.
-    SCase "v == v1".
-      assert (C : mem v (bind v1 t e1)).
-        apply mem_bind_same. rewrite beq_vid_sym. exact V.
-      apply compose_overlap
-        with (e1:=bind v1 t e1) (e2:=e2) (v:=v) in C.
-        rewrite C in H0; inversion H0.
-        exact H.
-    SCase "v /= v1".
+  Hint Resolve lookup_not_member.
+
+  Lemma not_mem_compose : forall (v : var) (e1 e2 e12 : env),
+    e1 & e2 = Some e12 ->
+    ~ (mem v e1) ->
+    ~ (mem v e2) ->
+    ~ (mem v e12).
+  Proof.
+    intros.
+    assert (L12 : lookup v e12 = lookup v e2); eauto.
+    assert (L2 : lookup v e2 = None); apply lookup_not_member; auto.
+    unfold mem, bmem. rewrite L12, L2. auto.
+  Qed.
+  Hint Resolve not_mem_compose.
+
+  Lemma compose_lookup_l : forall (e1 e2 e12 : env) (v : var),
+    mem v e1 ->
+    e1 & e2 = Some e12 ->
+    lookup v e12 = lookup v e1.
+  Proof.
+    intros.
+    generalize dependent e2. generalize dependent e12.
+    induction e1 as [ | v1 t e1].
+    Case "mtEnv".
+      apply mem_mtEnv in H. inversion H.
+    Case "bind v1 t1 e1". intros.
       apply bind_compose in H0.
       elim H0; intros; rename x into e; clear H0.
-      inversion H1; clear H1; subst.
-      rewrite lookup_bind_diff.
-        apply IHe1. exact H. exact H0.
-        exact V.
-Qed.
+      inversion_clear H1. subst.
+      destruct (beq_var_eq_dec v v1).
+    SCase "v == v1".
+      repeat rewrite H1. repeat rewrite lookup_bind_same; reflexivity.
+    SCase "v /= v1".
+      repeat rewrite lookup_bind_diff; auto.
+      apply IHe1 with (e2 := e2); auto.
+      apply mem_bind_diff with (v' := v1) (t := t); auto. 
+  Qed.
+  Hint Resolve compose_lookup_l.
 
-Lemma env_comm : forall (e1 e2 e12 e21 : env),
-  e1 & e2 = Some e12 -> e2 & e1 = Some e21 -> e12 ~= e21.
-Proof. 
-  intros e1 e2 e12 e21 H12 H21 v.
-  destruct (bmem v e1) eqn:V1; destruct (bmem v e2) eqn:V2;
-    try apply bmem_true in V1; try apply bmem_true in V2.
-  Case "v in e1, e2".
-    assert (C : e1 & e2 = None).
-      apply compose_overlap with (v := v). exact V1. exact V2.
-    rewrite C in H12. inversion H12.
-  Case "v in e1, not in e2".
-    assert (L12 : lookup v e12 = lookup v e1).
-      apply compose_lookup_l with (e2 := e2). exact V1. exact H12.
-    assert (L21 : lookup v e21 = lookup v e1).
-      apply compose_lookup_r with (e1 := e2). exact V1. exact H21.
-    rewrite L12. rewrite L21. reflexivity.
-  Case "v in e2, not in e1".
-    assert (L12 : lookup v e12 = lookup v e2).
-      apply compose_lookup_r with (e1 := e1). exact V2. exact H12.
-    assert (L21 : lookup v e21 = lookup v e2).
-      apply compose_lookup_l with (e2 := e1). exact V2. exact H21.
-    rewrite L12. rewrite L21. reflexivity.
-  Case "v not in e1, e2".
-    apply bmem_false in V1.
-    apply bmem_false in V2.
-    assert (L12 : lookup v e12 = lookup v e2).
-      apply compose_not_member with (e1 := e1). exact V1. exact H12.
-    assert (L21 : lookup v e21 = lookup v e1).
-      apply compose_not_member with (e1 := e2). exact V2. exact H21.
-    assert (L1 : lookup v e1 = pvar v).
-      apply lookup_not_member. exact V1.
-    assert (L2 : lookup v e2 = pvar v).
-      apply lookup_not_member. exact V2.
-    rewrite L12. rewrite L21. rewrite L1. rewrite L2. reflexivity.
-Qed.
+  Lemma compose_lookup_r : forall (e1 e2 e12 : env) (v : var),
+    mem v e2 ->
+    e1 & e2 = Some e12 ->
+    lookup v e12 = lookup v e2.
+  Proof.
+    intros.
+    generalize dependent e2. generalize dependent e12.
+    induction e1 as [ | v1 t e1].
+    Case "mtEnv". intros.
+      inversion H0. reflexivity.
+    Case "bind v1 t e1". intros.
+      destruct (beq_var_eq_dec v v1).
+    SCase "v == v1". 
+      assert (C : mem v (bind v1 t e1)).
+      apply mem_bind_same; auto.
+      apply compose_overlap
+        with (e1:=bind v1 t e1) (e2:=e2) (v:=v) in C; auto.
+      rewrite C in H0; inversion H0.
+    SCase "v /= v1".
+      apply bind_compose in H0.
+      inversion_clear H0 as (e & H2 & H3); subst.
+      rewrite lookup_bind_diff; auto.
+  Qed.
+  Hint Resolve compose_lookup_r.
 
-Lemma env_subs_comm : forall (e1 e2 e12 : env) (p : patt),
-  e1 & e2 = Some e12 ->
-  e12 * p = e1 * (e2 * p).
-Proof.
-  intros. induction p.
-  Case "var v".
-    destruct (bmem v e1) eqn:V1; destruct (bmem v e2) eqn:V2;
-      try apply bmem_true in V1; try apply bmem_true in V2.
-    SCase "v in e1, e2".
+  Lemma env_comm : forall (e1 e2 e12 e21 : env),
+    e1 & e2 = Some e12 -> e2 & e1 = Some e21 -> e12 == e21.
+  Proof. 
+    intros e1 e2 e12 e21 H12 H21 v.
+    destruct (bmem v e1) eqn:M1; destruct (bmem v e2) eqn:M2;
+      try apply bmem_true in M1; try apply bmem_true in M2.
+    Case "v in e1, e2".
       assert (C : e1 & e2 = None).
-        apply compose_overlap with (v := v). exact V1. exact V2.
-      rewrite C in H. inversion H.
-    SCase "v in e1, not in e2".
-      simpl. apply bmem_false in V2.
-      assert (L2 : lookup v e2 = pvar v).
-        apply lookup_not_member. exact V2.
-      assert (L12 : lookup v e12 = lookup v e1).
-        apply compose_lookup_l with (e2 := e2). exact V1. exact H.
-      rewrite L2. rewrite L12. simpl. reflexivity.
-    SCase "v in e2, not in e1".
-      simpl. apply bmem_false in V1.
-      assert (L12 : lookup v e12 = lookup v e2).
-        apply compose_lookup_r with (e1 := e1). exact V2. exact H.
-      assert (G : closed (lookup v e2)).
-        apply mem__subs_closed. exact V2.
-      apply closed_subs with (e := e1) in G.
-      rewrite G. rewrite L12. reflexivity.
-    SCase "v not in e1, e2".
-      simpl. apply bmem_false in V1. apply bmem_false in V2.
-      assert (L12 : lookup v e12 = lookup v e2).
-        apply compose_not_member with (e1 := e1). exact V1. exact H.
-      assert (L2 : lookup v e2 = pvar v).
-        apply lookup_not_member. exact V2.
-      assert (L1 : lookup v e1 = pvar v).
-        apply lookup_not_member. exact V1.
-      rewrite L12. rewrite L2. simpl. rewrite L1. reflexivity.
-  Case "node n nil".
-    reflexivity.
-  Case "node n (t :: ts)".
-    simpl. rewrite IHp.
-    inversion IHp0. rewrite H1.
-    reflexivity.
-Qed.
+      apply compose_overlap with (v := v). exact M1. exact M2.
+      rewrite C in H12. inversion H12.
+    Case "v in e1, not in e2".
+      transitivity (lookup v e1). eauto. symmetry; eauto.
+    Case "v in e2, not in e1".
+      transitivity (lookup v e2). eauto. symmetry; eauto.
+    Case "v not in e1, e2".
+      apply bmem_false in M1.
+      apply bmem_false in M2.
+      assert (M12 : ~ mem v e12); eauto. apply lookup_not_member in M12.
+      assert (M21 : ~ mem v e21); eauto. apply lookup_not_member in M21.
+      rewrite M12, M21; reflexivity.
+  Qed.
+  
+  Lemma env_join_concat : forall e1 e2 e12, 
+    e1 & e2 = Some e12 -> e12 = e1 ++ e2.
+  Proof.
+    induction e1. intros. inversion H. subst; auto.
+    intros. simpl in *.
+    destruct (bmem v e2); try discriminate.
+    destruct (e1 & e2) eqn:e12'.
+    apply IHe1 in e12'. subst. inversion H; auto. inversion H.
+  Qed.  
+
+  Lemma env_comm_2 : forall (e1 e2 e12 : env),
+    e1 & e2 = Some e12 -> exists e21, e2 & e1 = Some e21 /\ e12 == e21.
+  Proof.
+    intros. assert (H0 := H). assert (H1 := H).
+    apply env_join_concat in H0. 
+    apply concat_comm_equiv in H.
+    destruct (e2 & e1) eqn:e21. 
+    apply env_join_concat in e21. exists e. split; subst; auto. 
+    apply compose_overlap_2 in e21. inversion e21 as (x & H2 & H3). assert (H' := compose_overlap _ _ _ H3 H2).
+    rewrite H1 in H'. inversion H'.
+  Qed.
+
+End ENV.
