coq/Match.v
@@ -1,51 +1,480 @@
+Require Import Coq.Bool.Bool.
 Require Import Coq.Arith.EqNat.
 Require Import Coq.Lists.List.
+Require Import Coq.Classes.RelationClasses.
+Require Import Coq.Setoids.Setoid Coq.Classes.SetoidClass.
 Require Import Cases.
-Require Import Patt.
-Require Import Subs.
 Require Import Util.
-Import StdEnv.
+Require Import Env2.
+Require Import Term.
+Require Import Subs.
 
-Fixpoint pmatch (p : patt) (t : term) : option env :=
-  let pmatches := fix pmatches (ps : list patt) (ts : list term)
-    : option env :=
-      match (ts, ps) with
+Module Term.
+
+  Import StdEnv.
+(*
+  Module TermValue <: VALUE.
+    Definition val := term.
+    Definition var := var.
+    Definition beq_var := beq_nat.
+    Definition beq_var_refl := beq_var_refl.
+    Definition beq_var_sym := beq_var_sym.
+    Definition beq_var_trans := beq_var_trans.
+  End TermValue.
+
+  Module TVEnv := ENV(TermValue).
+  Import TVEnv.
+  Definition x := mtEnv.
+*)
+
+(*
+  Definition closed (t : term) : Prop :=
+    forall (v : var), fvar v t = false.
+
+  Definition term_rect := fun
+    (P : term -> Type)
+    (h : forall (v : var), P (tvar v))
+    (g : forall (n : id), P (node n nil))
+    (f : forall (n : id) (t : term) (ts : list term),
+      P t -> P (node n ts) -> P (node n (t :: ts)))
+    =>
+    fix term_rec (t : term) : P t :=
+    match t return P t with
+      | tvar v => h v
+      | node n ts =>
+        ((fix terms_rec (ts : list term) : P (node n ts) :=
+          match ts with
+            | nil => g n
+            | t :: ts => f n t ts (term_rec t) (terms_rec ts)
+          end) ts)
+    end.
+
+  Definition term_ind := fun
+    (P : term -> Prop)
+    (h : forall (v : var), P (tvar v))
+    (g : forall (n : id), P (node n nil))
+    (f : forall (n : id) (t : term) (ts : list term),
+      P t -> P (node n ts) -> P (node n (t :: ts)))
+    => term_rect P h g f.
+
+  Definition term_rec := fun
+    (P : term -> Set)
+    (h : forall (v : var), P (tvar v))
+    (g : forall (n : id), P (node n nil))
+    (f : forall (n : id) (t : term) (ts : list term),
+      P t -> P (node n ts) -> P (node n (t :: ts)))
+    => term_rect P h g f.
+*)
+
+  Fixpoint tmatch (q p : term) {struct q} : option env :=
+    let tmatches := fix tmatches (ps qs : list term) {struct qs} : option env :=
+      match (ps, qs) with
         | (nil, nil) => Some mtEnv
         | (nil, _) => None
         | (_, nil) => None
-        | (t :: ts, p :: ps) =>
-          e1 <- pmatch p t;
-          e2 <- pmatches ps ts;
-          compose_env e1 e2
+        | (p :: ps, q :: qs) =>
+          e1 <- tmatch q p;
+          e2 <- tmatches ps qs;
+          e1 & e2
       end in
-  match p with
-    | pvar v => Some (bind v t mtEnv)
-    | pnode n ps =>
-      match t with
-        | tnode n' ts =>
-          if negb (beq_nid n n')
-            then None
-            else pmatches ps ts
-      end
-  end.
+    match q with
+      | tvar v => Some (bind v p mtEnv)
+      | node n qs =>
+        match p with
+          | tvar _ => None
+          | node n' ps =>
+            if negb (beq_id n n')
+              then None
+              else tmatches ps qs
+          end
+    end.
 
-Notation "t / p" := (pmatch p t).
+  Notation "p / q" := (tmatch q p).
+
+
+  Lemma fvar_head : forall (t : term) (ts : list term) (n : id) (v : var),
+    fvar v t = true -> fvar v (node n (t :: ts)) = true.
+  Proof.
+    intros.
+    unfold fvar. apply orb_true_iff. left. fold fvar.
+    assumption.
+  Qed.
+
+  Lemma fvar_tail : forall (t : term) (ts : list term) (n : id) (v :var),
+    fvar v (node n ts) = true -> fvar v (node n (t :: ts)) = true.
+  Proof.
+    intros.
+    unfold fvar. apply orb_true_iff. right. fold fvar.
+    induction ts.
+      simpl in H. inversion H.
+      simpl in H. exact H.
+  Qed.
+
+  Lemma fvar_uncons : forall v n t ts,
+    fvar v (node n (t :: ts)) = true ->
+    fvar v t = true \/ fvar v (node n ts) = true.
+  Proof.
+    intros. simpl in H.
+    destruct (fvar v t).
+      left; reflexivity.
+      right. simpl in H.
+        destruct (fvar v (node n ts)) eqn:FV.
+          reflexivity.
+          simpl in FV. rewrite H in FV. inversion FV.
+  Qed.
+
+  Lemma closed_uncons : forall (t : term) (ts : list term) (n : id),
+    closed (node n (t :: ts)) -> closed t /\ closed (node n ts).
+  Proof.
+    intros. split; unfold closed in *;
+      intro v; specialize (H v);
+      unfold fvar in H; fold fvar in H;
+      apply orb_false_elim in H; inversion H; assumption.
+  Qed.
+
+  Lemma closed_subs : forall (t : term) (e : env),
+    closed t -> e * t = t.
+  Proof.
+    intros. induction t.
+    Case "tvar v".
+      unfold closed in H. specialize (H v).
+      simpl in H. rewrite beq_var_refl in H. inversion H.
+    Case "node nil".
+      reflexivity.
+    Case "node (t :: ts)".
+      simpl.
+      apply closed_uncons in H. inversion H.
+      apply IHt in H0. simpl. rewrite H0.
+      apply IHt0 in H1. simpl in H1. inversion H1.
+        rewrite H3. rewrite H3.
+      reflexivity.
+  Qed.
+
+  Lemma subs_nil : forall (e : env) (n : id),
+    e * node n nil = node n nil.
+  Proof. intros. reflexivity. Qed.
+  
+  Lemma subs_cons : forall (e : env) (t : term) (n : id) (ts : list term),
+    e * (node n (t :: ts)) =
+    node n (e * t :: map (subs e) ts).
+  Proof. reflexivity. Qed.
+
+  Lemma tmatch_cons : forall (n : id) (p q : term) (ps qs : list term) (a : env),
+    (node n (p :: ps)) / (node n (q :: qs)) = Some a ->
+    exists (b c : env),
+      (p / q = Some b /\
+      node n ps / node n qs = Some c /\
+      Some a = b & c).
+  Proof.
+    intros.
+    simpl in H. rewrite beq_id_refl in H. simpl in H.
+    destruct (p / q) as [b|].
+    Case "p / q = b".
+      destruct (node n ps / node n qs) as [c|] eqn:G;
+        simpl in G; rewrite beq_id_refl in G; simpl in G.
+      SCase "ps / qs = c".
+        exists b, c.
+        split; split; try reflexivity.
+        rewrite G in H. inversion H.
+        reflexivity.
+      SCase "ps / qs = None".
+        destruct ps eqn:P; destruct qs eqn:Q;
+          try inversion G; try inversion H.
+        rewrite G in H. simpl in H. inversion H.
+    Case "p / q = None".
+      inversion H.
+  Qed.
+  
+  Ltac break_ands :=
+    repeat match goal with 
+      | [ H : _ /\ _ |- _ ] => inversion H; clear H
+    end.
+  Ltac simpl_impls := 
+    repeat match goal with
+      | [ Imp : ?cond -> ?exp, Given : ?cond |- _ ] => 
+        let H' := fresh "H" in 
+          ((assert exp as H' by (apply Imp; exact Given)); try clear Imp)
+      | [ Given : ?cond, Imp : ?cond -> ?exp |- _ ] => 
+        let H' := fresh "H" in 
+          ((assert exp as H' by (apply Imp; exact Given)); try clear Imp)
+    end.
+  Ltac break_exists :=
+    repeat match goal with
+      | [ H : exists x, _ |- _] => elim H; intros; clear H
+    end.
+
+  Inductive TMatch (p q : term) (a : env) : Prop :=
+  | TMatch_var (v : var)
+    (Q : q = tvar v)
+    (A : a = bind v p mtEnv) : TMatch p q a
+  | TMatch_nil (n : id)
+    (P : p = node n nil)
+    (Q : q = node n nil)
+    (A : a = mtEnv) : TMatch p q a
+  | TMatch_cons (p0 q0 : term) (ps qs : list term) (n : id) (b c : env)
+    (P : p = node n (p0 :: ps))
+    (Q : q = node n (q0 :: qs))
+    (B : p0 / q0 = Some b)
+    (C : node n ps / node n qs = Some c)
+    (A : Some a = b & c) : TMatch p q a.
+
+  Lemma tmatch_case : forall (p q : term) (a : env),
+    p / q = Some a -> TMatch p q a.
+  Proof.
+    intros p.
+    induction q as [v | n | n q qs]; intros.
+    Case "q = tvar v".
+      apply TMatch_var with (v := v). reflexivity.
+      simpl in H. inversion H. reflexivity.
+    Case "q = node n nil".
+      induction p as [v | n' | n' p ps].
+      SCase "p = tvar v".
+        inversion H.
+      SCase "p = node n' nil".
+        simpl in H. destruct (beq_id n n') eqn:N.
+        SSCase "n == n'".
+          apply TMatch_nil with (n := n).
+            apply beq_id_true in N; rewrite N; reflexivity.
+          reflexivity.
+          inversion H; reflexivity.
+        SSCase "n /= n'".
+          inversion H.
+      SCase "p = node n' (p :: ps)".
+        simpl in H. destruct (beq_id n n'); inversion H.
+    Case "q = node n (q :: qs)".
+      induction p as [v | n' | n' p ps].
+      SCase "p = tvar v".
+        inversion H.
+      SCase "p = node n' nil".
+        simpl in H. destruct (beq_id n n'); inversion H.
+      SCase "p = node n' (p :: ps)".
+        clear IHp; clear IHp0.
+        destruct (beq_id n n') eqn:N.
+        SSCase "n == n'".
+          apply beq_id_true in N; symmetry in N; subst.
+          apply tmatch_cons in H.
+          inversion_clear H as (b & c & (B & C & A)).
+          eapply TMatch_cons; eauto.
+        SSCase "n /= n'".
+          inversion H as [H']; rewrite N in H'; inversion H'.
+  Qed.
+
+  (*
+  Lemma tmatch_ind' : forall (P : term -> term -> option env -> Prop),
+    (forall p v e, P p (tvar v) e) ->
+    (forall n e, P (node n nil) (node n nil) e) ->
+    (forall n p q ps qs, P (node n (p :: ps)) (node n (q :: qs))) ->
+    forall (p q : term), P p q.
+  Proof.
+    intros. simpl in *.
+    intros p.
+    induction q as [v | n | n q qs]; intros.
+    Case "q = tvar v".
+      apply TMatch_var with (v := v). reflexivity.
+      simpl in H. inversion H. reflexivity.
+    Case "q = node n nil".
+      induction p as [v | n' | n' p ps].
+      SCase "p = tvar v".
+        inversion H.
+      SCase "p = node n' nil".
+        simpl in H. destruct (beq_id n n') eqn:N.
+        SSCase "n == n'".
+          apply TMatch_nil with (n := n).
+            apply beq_id_true in N; rewrite N; reflexivity.
+          reflexivity.
+          inversion H; reflexivity.
+        SSCase "n /= n'".
+          inversion H.
+      SCase "p = node n' (p :: ps)".
+        simpl in H. destruct (beq_id n n'); inversion H.
+    Case "q = node n (q :: qs)".
+      induction p as [v | n' | n' p ps].
+      SCase "p = tvar v".
+        inversion H.
+      SCase "p = node n' nil".
+        simpl in H. destruct (beq_id n n'); inversion H.
+      SCase "p = node n' (p :: ps)".
+        clear IHp; clear IHp0.
+        destruct (beq_id n n') eqn:N.
+        SSCase "n == n'".
+          apply beq_id_true in N; symmetry in N; subst.
+          apply tmatch_cons in H.
+          inversion_clear H as (b & c & (B & C & A)).
+          eapply TMatch_cons; eauto.
+        SSCase "n /= n'".
+          inversion H as [H']; rewrite N in H'; inversion H'.
+  Qed.
+  *)
 
 (*
-Lemma fvar_pmatch : forall (v : vid) (t : term) (p : patt) (e : env),
-  t / p = Some e -> fvar v 
+  Lemma tmatch_inv : forall (p q : term) (a : env),
+    p / q = Some a ->
+      (exists (v : var), q = tvar v /\ a = bind v p mtEnv) \/
+      (exists (n : id), p = node n nil /\ q = node n nil) \/
+      (exists (p0 q0 : term) (ps qs : list term) (n : id) (b c : env),
+        p = node n (p0 :: ps) /\
+        q = node n (q0 :: qs) /\
+        p0 / q0 = Some b /\
+        node n ps / node n qs = Some c /\
+        Some a = b & c).
+  Proof.
+    intros. induction q as [v | n | n q qs].
+    Case "q = tvar v".
+      left.
+      exists v. split.
+        reflexivity.
+        simpl in H. inversion H. reflexivity.
+    Case "q = node n nil".
+      right. left.
+      induction p as [v | n' | n' p ps].
+      SCase "p = tvar v".
+        inversion H.
+      SCase "p = node n' nil".
+        simpl in H. destruct (beq_id n n') eqn:N.
+        SSCase "n == n'".
+          apply beq_id_true in N.
+          exists n. split; rewrite N; reflexivity.
+        SSCase "n /= n'".
+          inversion H.
+      SCase "p = node n' (p :: ps)".
+        simpl in H. destruct (beq_id n n'); inversion H.
+    Case "q = node n (q :: qs)".
+      right. right.
+      clear IHq; clear IHq0.
+      induction p as [v | n' | n' p ps].
+      SCase "p = tvar v".
+        inversion H.
+      SCase "p = node n' nil".
+        simpl in H. destruct (beq_id n n'); inversion H.
+      SCase "p = node n' (p :: ps)".
+        clear IHp; clear IHp0.
+        destruct (beq_id n n') eqn:N.
+        SSCase "n == n'".
+          apply beq_id_true in N; symmetry in N; subst.
+          apply tmatch_cons in H.
+          inversion_clear H as (b & c & H0).
+          exists p, q, ps, qs, n, b, c. auto.
+        SSCase "n /= n'".
+          inversion H as [H']; rewrite N in H'; inversion H'.
+  Qed.
 *)
 
-Definition subpattern (p q : patt) : Prop :=
-  exists (e : env), e * p = q.
+  Lemma subs_tmatch_comm : forall (p q : term) (a p_q ap_q a_pq : env),
+    (forall (x : var), mem x a -> fvar x q = true) ->
+    (a * p) / q = Some ap_q ->
+    p / q = Some p_q ->
+    a & p_q = Some a_pq ->
+    a_pq == ap_q.
+  Proof.
+    (*
+    intros p q a p_q ap_q a_pq M AP_Q PQ A_PQ.
+    assert (H := tmatch_case p q p_q). simpl_impls.
+    inversion H0.
+    Case "q = tvar v". rename v into vq.
+      simpl in *. intro.
+      inversion AP_Q; clear AP_Q. inversion PQ; clear PQ. subst.
+      admit.
+    Case "q = node n nil".
+      simpl; intro. subst.
+      simpl in AP_Q. rewrite beq_id_refl in AP_Q. simpl in AP_Q.
+      inversion AP_Q. subst.
+      assert (H: a = mtEnv).
+        destruct a. reflexivity.
+        specialize M with v0. simpl in M.
+        assert (false = true). apply M. apply mem_bind. inversion H.
+      rewrite H in A_PQ. inversion A_PQ.
+      subst; reflexivity.
+    Case "q = node n (q :: qs)".
+      intro; subst.
+      rename q0 into q. rename p0 into p.
+      induction q.
+      apply tmatch_cons in PQ.
+      simpl in *. rewrite beq_id_refl in *. simpl in *.
+      *)
+      
 
-Notation "p <= q" := (subpattern p q).
+    intros p q a p_q ap_q a_pq M AP_Q PQ A_PQ.
+    generalize dependent p.
+    induction q as [v | n | n q qs]; intros p AP_Q PQ.
+    Case "q = var v".
+      simpl in *.
+      inversion AP_Q; clear AP_Q. inversion PQ; clear PQ. subst.
+      admit.
+    Case "q = node n nil". (* implies p = node n nil, a = mtEnv *)
+      induction p.
+      SCase "p = tvar".
+        inversion PQ.
+      SCase "p = node n nil".
+        simpl in M. destruct a as [|v t a].
+        SSCase "a = mtEnv". (* trivial *)
+          simpl in *. rewrite AP_Q in PQ.
+          inversion PQ; inversion A_PQ; subst.
+          intro. reflexivity.
+        SSCase "a = bind v t a". (* impossible *)
+          assert (C: mem v (bind v t a)). apply mem_bind. 
+          assert (C: mem v (bind v t a)) by (apply mem_bind).
+          apply M in C. inversion C.
+      SCase "p = node n (p :: ps)".
+        clear IHp; clear IHp0.
+        simpl in PQ.
+        destruct (negb (beq_id n n0)); inversion PQ.
+    Case "q = node n (q :: qs)".
+      induction p as [v' | n' | n' p ps]. (* p = node n (p :: ps) *)
+      SCase "p = tvar".
+        simpl in PQ. inversion PQ.
+      SCase "p = node n' nil".
+        simpl in PQ. destruct (negb (beq_id n n')); inversion PQ.
+      SCase "p = node n' (p :: ps)".
+        clear IHp; clear IHp0.
+        rewrite subs_cons in AP_Q.
+        destruct (beq_id n n') eqn:N.
+        SSCase "n == n'".
+          apply beq_id_true in N; subst.
+          apply tmatch_cons in PQ. inversion PQ.
+          apply tmatch_cons in AP_Q.
+          break_exists. break_ands.
+          rewrite H3 in H5; inversion H5; subst; clear H5.
+          rewrite H0 in H1; inversion H1; subst; clear H1; clear H8.
+          intro.
+          assert (FV : forall v,
+            mem v a -> fvar v q = true \/ fvar v (node n' qs) = true) by
+            (intros v0 Mem; apply M in Mem; apply fvar_uncons in Mem; exact Mem).
+          
+          eapply IHq0.
+            admit. (* false *)
+            
+            intros. apply FV in H1. elim H1; intro.
+              eapply fvar_head in H5
+            assumption.
+            (* Why doesn't 
+          eapply IHq0.
+            intros. apply M in H1.
+            
+          
+          
+        SSCase "n /= n'".
+          simpl in PQ. rewrite N in PQ. inversion PQ.
+  Qed.
 
-Lemma subpattern_refl : forall (p : patt), p <= p.
-Proof.
-  intros. unfold subpattern. exists mtEnv. apply mtEnv_subs_l.
-Qed.
+  Lemma prime : forall (p q r : term) (a b c : env),
+    (a * p) / q = Some b -> p / q = Some c -> b * r = a * (c * r).
+  Proof.
+    intros.
 
-Lemma pmatch_subs : forall (t : term) (p : patt) (e : env),
-  t / p = Some e -> e * p = term_to_patt t.
-Proof.
+  (* false *)
+  (*
+  Lemma subs_assoc : forall (t : term) (e1 e2 : env),
+    (e2 ++ e1) * t = e1 * (e2 * t).
+  Proof.
+    intros. induction t.
+    Case "tvar". simpl.
+      destruct (lookup v e2) eqn:V.
+        apply lookup_concat_member with (e2 := e1) in V. rewrite V.
+  *)      
+
+  Lemma match_subs : forall (p q : term) (v : var) (e : env),
+    p / q = Some e -> e * q = p.
+  Proof.
+    intros.
+
+End Term.
