coq/Term.v
@@ -1,118 +1,91 @@
+Require Import Coq.Bool.Bool.
 Require Import Coq.Arith.EqNat.
 Require Import Coq.Lists.List.
 Require Import Cases.
 
-(*
-
-
-!!! Replaced by Patt.v !!!
-
-
-*)
-
-Definition vid := nat.
-Definition nid := nat.
-Definition beq_vid := beq_nat.
-Definition beq_nid := beq_nat.
+Definition var := nat.
+Definition id := nat.
+Definition beq_var := beq_nat.
+Definition beq_id := beq_nat.
 
 Unset Elimination Schemes.
 Inductive term :=
-| var : vid -> term
-| node : nid -> list term -> term. 
+| tvar : var -> term
+| node : id -> list term -> term.
 Set Elimination Schemes.
 
-Definition term_ind := fun
-  (P : term -> Prop)
-  (h : forall (v : vid), P (var v))
-  (g : forall (n : nid), P (node n nil))
-  (f : forall (n : nid) (t : term) (ts : list term),
+Fixpoint fvar (v : var) (t : term) : bool :=
+  match t with
+    | tvar v' => beq_var v v'
+    | node _ ts =>
+      (fix fvars (ts : list term) : bool :=
+        match ts with
+          | nil => false
+          | t :: ts => fvar v t || fvars ts
+        end) ts
+  end.
+
+Definition closed (t : term) : Prop :=
+  forall (v : var), fvar v t = false.
+
+(* Term Induction *)
+
+Definition term_rect := fun
+  (P : term -> Type)
+  (h : forall (v : var), P (tvar v))
+  (g : forall (n : id), P (node n nil))
+  (f : forall (n : id) (t : term) (ts : list term),
     P t -> P (node n ts) -> P (node n (t :: ts)))
   =>
   fix term_rec (t : term) : P t :=
-    match t return P t with
-      | var v => h v
-      | node n ts =>
-        ((fix terms_rec (ts : list term) : P (node n ts) :=
-          match ts with
-            | nil => g n
-            | t :: ts => f n t ts (term_rec t) (terms_rec ts)
-          end) ts)
-    end.
-
-(*
-Definition term_ind_base := fun
-  (P : term -> Prop)
-  (h : forall (v : vid), P (var v))
-  (f : forall (n : nid) (ts : list term), Forall P ts -> P (node n ts))
-  =>
-  fix term_rec (p : term) : P p :=
-    match p return P p with
-      | var v => h v
-      | node n ps =>
-      f n ps ((fix terms_rec (ps : list term) : Forall P ps :=
-        match ps with
-          | nil => Forall_nil P
-          | p :: ps => Forall_cons p (term_rec p) (terms_rec ps)
-        end) ps)
-    end.
-
-Lemma term_ind
-  (P : term -> Prop)
-  (h : forall (v : vid), P (var v))
-  (g : forall (n : nid), P (node n nil))
-  (f : forall (n : nid) (t : term) (ts : list term),
-    P t -> P (node n ts) -> P (node n (t :: ts)))
-  : forall (t : term), P t.
-Proof.
-  intros. induction t using term_ind_base.
-  Case "var". exact (h v).
-  Case "node n ts". clear h. induction ts.
-    SCase "nil". exact (g n).
-    SCase "t :: ts". apply f.
-      inversion H; subst. exact H2.
-      inversion H; subst. exact (IHts H3).
-Qed.
-*)
-
-
-
-Lemma beq_nid_refl : forall (n : nid), beq_nid n n = true.
-Proof. intros. unfold beq_nid. rewrite (beq_nat_refl n). reflexivity. Qed.
-
-Lemma beq_vid_refl : forall (v : vid), beq_vid v v = true.
-Proof. intros. unfold beq_vid. rewrite (beq_nat_refl v). reflexivity. Qed.
-
-Lemma beq_vid_true : forall x y : vid, beq_vid x y = true -> x = y.
-Proof. intros. unfold beq_nid. apply beq_nat_true. assumption. Qed.
-
-(*
-
-Inductive fixedTerm {r : Type} :=
-| fixedVar : vid -> fixedTerm
-| fixedNode : nid -> list r -> fixedTerm.
-
-Fixpoint term_fixpoint {r : Type}
-  (f : fixedTerm -> r) (t : term) : r :=
-  match t with
-    | var v => f (fixedVar v)
-    | node n ts => f (fixedNode n (map (term_fixpoint f) ts))
-  end.
-
-Fixpoint termSize2 (t : term) : nat :=
-  term_fixpoint (fun (t : fixedTerm) =>
-    match t with
-      | fixedVar _ => 0
-      | fixedNode _ ns => fold_left plus ns 0
-    end) t.
-
-Fixpoint termSize1 (t : term) : nat :=
-  match t with
-    | var v => 0
-    | node _ ts =>
-      ((fix termSizes (ts : list term) :=
+  match t return P t with
+    | tvar v => h v
+    | node n ts =>
+      ((fix terms_rec (ts : list term) : P (node n ts) :=
         match ts with
-          | nil => 0
-          | t :: ts => termSizes ts + termSize1 t
+          | nil => g n
+          | t :: ts => f n t ts (term_rec t) (terms_rec ts)
         end) ts)
   end.
-*)
+
+Definition term_ind := fun
+  (P : term -> Prop)
+  (h : forall (v : var), P (tvar v))
+  (g : forall (n : id), P (node n nil))
+  (f : forall (n : id) (t : term) (ts : list term),
+    P t -> P (node n ts) -> P (node n (t :: ts)))
+  => term_rect P h g f.
+
+Definition term_rec := fun
+  (P : term -> Set)
+  (h : forall (v : var), P (tvar v))
+  (g : forall (n : id), P (node n nil))
+  (f : forall (n : id) (t : term) (ts : list term),
+    P t -> P (node n ts) -> P (node n (t :: ts)))
+  => term_rect P h g f.
+
+(* Lemmas *)
+
+Lemma beq_var_refl : forall (x : var),
+  beq_var x x = true.
+Proof. intro. rewrite <- beq_nat_refl. reflexivity. Qed.
+
+Lemma beq_var_sym : forall (x y : var),
+  beq_var x y = beq_var y x.
+Proof. exact NPeano.Nat.eqb_sym. Qed.
+
+Lemma beq_var_trans : forall (x y z : var),
+  beq_var x y = true -> beq_var y z = true -> beq_var x z = true.
+Proof.
+  intros. unfold beq_var in *.
+  apply beq_nat_true in H. rewrite H. exact H0.
+Qed.
+
+Lemma beq_var_true : forall x y : var, beq_var x y = true -> x = y.
+Proof. intros. apply beq_nat_true. assumption. Qed.
+
+Lemma beq_id_refl : forall (n : id), beq_id n n = true.
+Proof. intros. rewrite (beq_nat_refl n). reflexivity. Qed.
+
+Lemma beq_id_true : forall x y : id, beq_id x y = true -> x = y.
+Proof. intros. apply beq_nat_true. assumption. Qed.
